prepare stack demo

examples/Stack/Stack.ml
@@ -1,0 +1,32 @@
+
+(** Implementation of a stack using lists *)
+
+type 'a stack = ('a list) ref
+
+let create () =
+  ref []
+
+let is_empty p =
+  !p = []
+
+let push p x =
+  p := x :: !p
+
+let pop p =
+  match !p with
+  | [] -> raise Not_found
+  | x::r -> p := r; x
+
+let clear p =
+  p := []
+
+let concat p1 p2 =
+  p1 := !p1 @ !p2;
+  clear p2
+
+let rev_append f p1 p2 =
+  if not (is_empty p1) then begin
+    let x = pop p1 in
+    push p2 x;
+    f p1 p2
+  end
