examples/Stack/StackSized.ml
@@ -1,0 +1,37 @@
+
+(** Implementation of a stack using lists and storing the size *)
+
+type 'a t = {
+   mutable items : 'a list;
+   mutable size : int }
+
+let create () =
+  { items = [];
+    size = 0 }
+
+let size s =
+  s.size
+
+let is_empty s =
+  s.size = 0
+
+let push x s =
+  s.items <- x :: s.items;
+  s.size <- s.size + 1
+
+let pop s =
+  match s.items with
+  | hd::tl ->
+      s.items <- tl;
+      s.size <- s.size - 1;
+      hd
+  | [] -> assert false
+
+let clear p =
+  p.data <- [];
+  p.size <- 0
+
+let concat p1 p2 =
+  p1.data <- p1.data @ p2.data;
+  p1.size <- p1.size + p2.size;
+  clear p2
