examples/Tutorial/OldTutorial.ml
@@ -1,0 +1,193 @@
+
+
+
+(***********************************************************************)
+(** Basic operations *)
+
+let example_let n =
+  let a = n+1 in
+  let b = n-1 in
+  a + b
+
+let example_incr r =
+  r := !r + 1
+
+let example_two_ref n =
+  let i = ref 0 in
+  let r = ref n in
+  decr r;
+  incr i;
+  r := !i + !r;
+  !i + !r
+
+
+(***********************************************************************)
+(** For loops *)
+
+let facto_for n =
+  let r = ref 1 in
+  for i = 1 to n do
+    r := !r * i;
+  done;
+  !r
+
+let fib_for n =
+  let a = ref 0 in
+  let b = ref 1 in
+  for i = 0 to n-1 do
+    let c = !a + !b in
+    a := !b;
+    b := c;
+  done;
+  !a
+
+
+(***********************************************************************)
+(** While loops *)
+
+let example_while n =
+  let i = ref 0 in
+  let r = ref 0 in
+  while !i < n do
+    incr i;
+    incr r;
+  done;
+  !r
+
+let facto_while n =
+  let r = ref 1 in
+  let i = ref 2 in
+  while !i <= n do
+    r := !i * !r;
+    incr i;
+  done;
+  !r
+
+let is_prime n =
+  let i = ref 2 in
+  let p = ref true in
+  while !p && (!i * !i <= n) do
+    if (n mod !i) = 0
+      then p := false;
+    incr i;
+  done;
+  !p
+
+
+(***********************************************************************)
+(** Recursion *)
+
+let rec facto_rec n =
+  if n <= 1
+    then 1
+    else n * facto_rec(n-1)
+
+let rec fib_rec n =
+  if n <= 1
+    then n
+    else fib_rec(n-1) + fib_rec(n-2)
+
+
+(***********************************************************************)
+(** Stack *)
+
+module StackList = struct
+
+  type 'a t = {
+     mutable items : 'a list;
+     mutable size : int }
+
+  let create () =
+    { items = [];
+      size = 0 }
+
+  let size s =
+    s.size
+
+  let is_empty s =
+    s.size = 0
+
+  let push x s =
+    s.items <- x :: s.items;
+    s.size <- s.size + 1
+
+  let pop s =
+    match s.items with
+    | hd::tl ->
+        s.items <- tl;
+        s.size <- s.size   - 1;
+        hd
+    | [] -> assert false
+
+end
+
+
+(***********************************************************************)
+(** Array *)
+
+let demo_array () =
+  let t = Array.make 3 true in
+  t.(0) <- false;
+  t.(1) <- false;
+  t
+
+let exercise_array () =
+  let t = Array.make 3 true in
+  t.(2) <- false;
+  t.(1) <- t.(2);
+  t
+
+
+(***********************************************************************)
+(** Vector *)
+
+(* Futur work
+
+module Vector = struct
+
+  type 'a t = {
+    mutable data : 'a array;
+    mutable size : int;
+    default: 'a; }
+
+  let create size def =
+    { data = Array.make size def;
+      size = size;
+      default = def; }
+
+  let size t =
+    t.size
+
+  let get t i =
+    t.data.(i)
+
+  let set t i v =
+    t.data.(i) <- v
+
+  let double_size t =
+    let src = t.data in
+    let size = t.size in
+    let size2 = 2 * size in
+    let dst = Array.make size2 t.default in
+    for i = 0 to pred size do
+      dst.(i) <- src.(i);
+    done
+
+  let push t v =
+    let size = t.size in
+    let capa = Array.length t.data in
+    if size = capa
+      then double_size t;
+    t.size <- size+1;
+    t.data.(size) <- v
+
+end
+
+*)
+
+(* Variants for double_size t:
+   Array.iteri (fun i v <- dst.(i) <- v) src
+   Array.init size2 (fun i -> if i < size then src.(i) else t.default)
+*)
+
+
