examples/Tutorial/Tutorial_proof.v
@@ -1,828 +1,490 @@
+
+
 Set Implicit Arguments.
-Require Import CFML.CFLib.
-Require Import Stdlib.
-Require Import Array_proof.
-Require Import Tuto_ml.
-Require Import TLC.LibListZ.
+From Sep Require Import Example.
+From Sep Require ExampleStack ExampleList.
+Generalizable Variables A.
+
+Implicit Types n m : int.
+Implicit Types p q : loc.
 
 
-(***********************************************************************)
-(** Cheat list *)
+(* ####################################################### *)
+(** * Basic programs *)
 
-(**
-Specification syntax:
-   - [app f [x y]
-        PRE H
-        POST (fun (x:T) => H']
-
-Heap syntax H :  heap -> Prop ::=
-   - \[]
-   - \[P]
-   - H \* H'
-   - r ~~> v        r ~> Ref v       Ref v r
-   - r ~~> (v+1)
-   - Hexists x, H
-   - r ~> Stack L       Stack L r
-
-Coq tactics:
-   - [=> x], [=>> H], [exists v]
-   - [rew_maths] for normalizing math expressions
-   - [rew_list] for normalizing list operations
-   - [autos], [math], [ring], [math_nia]
-
-CFML tactics:
-   - [xcf]
-   - [xsimpl], or [xsimpl X1 .. X2] (to instantiate Hexists)
-   - [xpull]
-   - [xclean] sometimes needed to do simplifications
-   - [xret], or [xrets] for substitution/simplification
-   - [xapp], or [xapps] for substitution
-   - [xfor_inv (fun i => H)]
-   - [xwhile_inv_basic (fun b k => [b = isTrue(..)] \* H) (downto n)]
-   - [xif Q]
-   - [xmatch]
-
-Shortcut:
-   - [xextracts] like [xextract; intros x; subst x]
-   - [xrets] like [xret; xsimpl]
-   - [xapps] like [xapp; xextracts]
-   - [tactic~] like [tactic; eauto with maths]
-*)
+Module Basics.
 
 
-(***********************************************************************)
-(** Mathematical definitions *)
-
-(** Factorial *)
-
-Parameter facto : int -> int.
-Parameter facto_zero : facto 0 = 1.
-Parameter facto_one : facto 1 = 1.
-Parameter facto_succ : forall n, n >= 1 -> facto n = n * facto(n-1).
-
-(** Fibonnaci *)
-
-Parameter fib : int -> int.
-Parameter fib_base : forall n, n <= 1 -> fib n = n.
-Parameter fib_succ : forall n, n > 1 -> fib n = fib(n-1) + fib(n-2).
-
-(** Primes *)
-
-Parameter prime : int -> Prop.
-Parameter divide_not_prime : forall n d,
-  1 < d < n ->
-  Z.rem n d = 0 ->
-  ~ (prime n).
-Parameter not_divide_prime : forall n,
-  (forall d, 1 < d < n -> Z.rem n d <> 0) ->
-  (prime n).
-Parameter not_divide_prime_sqrt : forall n r,
-  (forall d, 1 < d < r -> Z.rem n d <> 0) ->
-  (r * r > n) ->
-  (prime n).
-
-
-(***********************************************************************)
-(** Automation for mathematical subgoals *)
-
-Ltac auto_tilde ::= try solve [ intuition eauto with maths ].
-  (* TODO: try to use jauto *)
-
-Hint Extern 1 (index ?M _) => subst M : maths.
-Hint Resolve LibListZ.index_make : maths.
-Hint Resolve index_of_inbound : maths.
-Hint Resolve index_of_index_length int_index_prove : maths.
-Hint Resolve index_update : maths.
-
-(** Tactic [rew_maths] for simplifying math expressions *)
-
-Lemma math_plus_one_twice : forall n, ((n+1)+1) = n+2.
-Proof using. math. Qed.
-Lemma math_minus_same : forall n, n-n = 0.
-Proof using. math. Qed.
-Lemma math_two_minus_one : 2-1 = 1.
-Proof using. math. Qed.
-Lemma math_plus_minus_same : forall n m, (n+m)-m = n.
-Proof using. math. Qed.
-Hint Rewrite math_plus_one_twice math_minus_same
-  math_two_minus_one math_plus_minus_same : rew_maths.
-
-
-
-
-
-(***********************************************************************)
-(** Basic operations *)
-
-(*---------------------------------------------------------------------*)
+(* ******************************************************* *)
+(** *** Let computation *)
 
 (**
 [[
   let example_let n =
-    let a = n+1 in
-    let b = n-1 in
+    let a = n + 1 in
+    let b = n - 1 in
     a + b
 ]]
 *)
 
-Lemma example_let_spec : forall n,
-  app example_let [n]
+Definition example_let :=
+  Fun 'n :=
+    Let 'a := 'n '+ 1 in
+    Let 'b := 'n '- 1 in
+    'a '+ 'b.
+
+Lemma Triple_example_let : forall n,
+  TRIPLE (example_let n)
     PRE \[]
-    POST (fun (v:int) => \[v = 2*n]).
-   (* post-condition also written: POST \[= (2 * n)]  *)
+    POST (fun r => \[r = 2*n]).
 Proof using.
-  (* Hint: the proof uses [xcf], [xret], [xsimpl], [math].
-     [xlet] is optional; if used then [xpull] is also needed. *)
-  dup 3.
-  { (* detailed proof *)
-    xcf.
-    xlet. xret. simpl. xpull. intros Ha.
-    xlet. xret. simpl. xpull. intros Hb.
-    xret. (*hnf.*) xsimpl. math. }
-  { (* shorter proof *)
-    xcf. xret ;=> Ha. xret ;=> Hb. xret. xsimpl. math. }
-  { (* real proof *)
-    xcf. xrets. xrets. xrets. math. }
+  xwp. xapp. xapp. xapp. xsimpl. math.
 Qed.
 
+(** Note: [xapp] calls [xlet] automatically when needed. *)
 
-(*---------------------------------------------------------------------*)
+(** Note: [xappn] factorizes the [xapp] calls. *)
+
+(** Note: [xsimpl*] does [xsimpl] but automation that can call [xmath]. *)
+
+
+(* ******************************************************* *)
+(** *** Increment *)
 
 (**
 [[
-  let example_incr r =
-    r := !r + 1
-]]
-
-normalized to:
-
-[[
-  let example_incr r =
-    let x0__ := get r in
-    set r (x0__ + 1)
+  let incr p =
+    p := !p + 1
 ]]
 *)
 
-Lemma example_incr_spec : forall r n,
-  app example_incr [r]
-    PRE (r ~~> n)
-    POST (fun (_:unit) => (r ~~> (n+1))).
-    (* post-condition also written: POST (# r ~~> (n+1)). *)
+Definition incr : val :=
+  Fun 'p :=
+   'p ':= '! 'p '+ 1.
+
+Lemma Triple_incr : forall (p:loc) (n:int),
+  TRIPLE (incr p)
+    PRE (p ~~> n)
+    POST (fun (r:unit) => (p ~~> (n+1))).
 Proof using.
-  (* Hint: the proof uses [xcf], [xapp].
-     [xapps] is a shortand for [xapp] followed with [subst]. *)
-  dup 3.
-  { xcf. xlet. xapp. simpl. xpull. intros. subst. xapp. }
-  { xcf. xapp. intros. subst. xapp. }
-  { xcf. xapps. xapp. }
+  xwp. xapp. xapp. xapp. xsimpl.
 Qed.
 
-(* Note: recall the specifications of get and set from Pervasives_proof:
+Hint Extern 1 (Register_Spec (incr)) => Provide Triple_incr.
 
-  Lemma get_spec : forall A (v:A) r,
-    app get [r]
-      PRE (r ~~> v)
-      POST (fun x => \[x = v] \* r ~~> v)
 
-  Lemma set_spec : forall A (v w:A) r,
-    app set [r w] (r ~~> v) (# r ~~> w).
-
-*)
-
-(*---------------------------------------------------------------------*)
+(* ******************************************************* *)
+(** *** Successor using increment *)
 
 (**
 [[
-let example_two_ref n =
-  let i = ref 0 in
-  let r = ref n in
-  decr r;
-  incr i;
-  r := !i + !r;
-  !i + !r
-]]
-*)
-
-Lemma example_two_ref_spec : forall n: int,
-  (* <EXO> *)
-  app example_two_ref [n]
-     PRE \[]
-     POST (fun x: int => \[ x = n+1 ]).
-  (* </EXO *)
-Proof using.
-  (* Hint: the proof uses [xcf], [xapp], [xapps], and [xret] or [xrets]. *)
-  dup 3.
-  { (* detailed proof *)
-    xcf.
-    xapp. (* details: xlet. xapp. simpl. *)
-    xapp. xapp. xapp.
-    xapps. (* details: xapp. intro. subst. *)
-    xapps. xapps. xapps. xapps.
-    xrets. (* details: xret. xsimpl. *)
-    math. }
-  { (* shorter proof, not recommended for nontrivial code *)
-    xcf. xgo. subst. math. }
-  { (* real proof *)
-    xcf. xgo~. }
-Qed.
-
-
-
-(***********************************************************************)
-(** For loops *)
-
-(*---------------------------------------------------------------------*)
-
-(**
-[[
-  let facto_for n =
-    let r = ref 1 in
-    for i = 1 to n do
-      r := !r * i;
-    done;
-    !r
-]]
-*)
-
-(* Reasoning principle for the loop [for i = a to b to t done] when [b+1>=a]
-   implemented by tactic [xfor_inv I].
-
-  I a               initial invariant
-
-  I i -> I (i+1)    when executing [t] on some [i] in the range from [a] to [b]
-
-  I (b+1)           final invariant
-
-*)
-
-Lemma facto_for_spec : forall n,
-  n >= 1 ->
-  app facto_for [n]
-    PRE \[]
-    POST (fun (v:int) => \[v = facto n]).
-Proof using.
-  =>> Hn. xcf. xapps.
-  xfor_inv (fun i => r ~~> (facto (i-1))).
-  { math. }
-  { xsimpl. forwards: facto_zero. easy. }
-  { =>> Hi. xapps. xapps. xsimpl.
-    rew_maths. rewrite (@facto_succ i). ring. math. }
-  xapps. xsimpl. rew_maths. auto.
-Qed.
-
-
-
-(*---------------------------------------------------------------------*)
-
-(**
-[[
-  let fib_for n =
-    let a = ref 0 in
-    let b = ref 1 in
-    for i = 0 to n-1 do
-      let c = !a + !b in
-      a := !b;
-      b := c;
-    done;
-    !a
-]]
-*)
-
-Lemma fib_for_spec : forall n,
-  n >= 1 ->
-  app fib_for [n]
-    PRE \[]
-    POST (fun (v:int) => \[v = fib n]).
-Proof using.
-  (* Hint: follow the pattern from the previous example *)
-  (* <EXO> *)
-  =>> Hn. xcf. xapps. xapps.
-  xfor_inv (fun i => a ~~> (fib i) \* b ~~> (fib (i+1)) ).
-  { math. }
-  { xsimpl.
-    rewrite~ fib_base. (* details: math. math. rewrite fib_base. *)
-    rewrite~ fib_base. }
-  { =>> Hi. xapps. xapps. xrets. xapps. xapps. xapps. xsimpl.
-    rew_maths. rewrite~ (@fib_succ (i+2)). rew_maths.
-    math_rewrite ((i + 2)-1 = i+1). math. }
-  xapps. xsimpl~.
-  (* </EXO> *)
-Qed.
-
-
-(*----Alternative script:
-
-  =>> Hn. xcf. xapps. xapps.
-  xfor_inv (fun i => a ~~> (fib i) \* b ~~> (fib (i+1))).
-  { math. }
-  { xsimpl.
-    { forwards~: fib_base. math. }
-    { forwards~: fib_base. math. } }
-  { introv Hi. xapps. xapps. xret. intros. xapps. xapps. xapps. xsimpl.
-    rewrite fib_succ. rew_maths. math. math. }
-  xapps. xsimpl. auto.
-*)
-
-
-
-(***********************************************************************)
-(** While loops *)
-
-(*---------------------------------------------------------------------*)
-
-(**
-[[
-  let example_while n =
-    let i = ref 0 in
-    let r = ref 0 in
-    while !i < n do
-      incr i;
-      incr r;
-    done;
-    !r
-]]
-*)
-
-(* Reasoning principle for the loop [while t1 do t2] using an invariant
-   implemented by tactic [xwhile_inv_basic J W].
-
-  J b i             true for some boolean [b] and some initial index [k]
-
-  J b i             when executing [t1] on some [i]
-   ->
-  J b' i
-
-  J true i          when executing [t2] on some [i], should restablish the
-   ->               invariant for some [b'] and some [i'] smaller than [i]
-  J b' i'           w.r.t. [W], that is [W i' i].
-
-  J false i         for some [i] describes the final state
-
-*)
-
-
-Lemma example_while_spec : forall n,
-  n >= 0 ->
-  app example_while [n]
-    PRE \[]
-    POST (fun (v:int) => \[v = n]).
-Proof using.
-  introv Hn. xcf. xapps. xapps.
-  xwhile_inv_basic (fun b k => \[b = isTrue (k < n)] \* \[k <= n] \* i ~~> k \* r ~~> k)
-    (upto n).
-  { xsimpl. eauto. eauto. }
-  { => b k. xpull. => Hb Hk. xapps. xrets. auto. autos*. } (* short for: xret; xsimpl. *)
-  { => k. xpull. => Hb Hk. xapps. xapps. xsimpl.
-    { math. }
-    { eauto. }
-    { hnf. math. } }
-  =>> Hb Hk. xclean. xapps. xsimpl. subst. math.
-Qed.
-
-
-(*---------------------------------------------------------------------*)
-
-(**
-[[
-  let facto_while n =
-    let r = ref 1 in
-    let i = ref 1 in
-    while !i <= n do
-      r := !i * !r;
-      incr i;
-    done;
-    !r
-]]
-*)
-
-Lemma facto_while_spec : forall n,
-  n >= 2 ->
-  app facto_while [n]
-    PRE \[]
-    POST (fun (v:int) => \[v = facto n]).
-Proof using.
-  (* Hint: follow the pattern from previous example *)
-  (* <EXO> *)
-  introv Hn. xcf. xapps. xapps.
-  xwhile_inv_basic (fun b k => \[b = isTrue (k <= n)] \* \[2 <= k <= n+1]
-                               \* i ~~> k \* r ~~> (facto (k-1)))
-    (upto (n+1)).
-  { xsimpl. rew_maths. rewrite~ facto_one. math. eauto. }
-  { => b k. xpull. => Hb Hk. xapps. xrets. auto. autos*. } (* short for: xret; xsimpl. *)
-  { => k. xpull. => Hb Hk. xapps. xapps. xapps. xapps. xsimpl.
-    { rew_maths. rewrite (@facto_succ k). ring. math. }
-    { math. }
-    { eauto. }
-    { math. } }
-  =>> Hb Hk. xclean. xapps. xsimpl. subst. fequal. math.
-  (* </EXO> *)
-Qed.
-
-
-(*---------------------------------------------------------------------*)
-
-(* TODO: add demos using the other xfor and xwhile approach *)
-
-(*---------------------------------------------------------------------*)
-
-(**
-[[
-  let is_prime n =
-    let i = ref 2 in
-    let p = ref true in
-    while !p && (!i * !i <= n) do
-      if (n mod !i) = 0
-        then p := false;
-      incr i;
-    done;
+  let succ_using_incr n =
+    let p = ref n in
+    incr p;
     !p
 ]]
 *)
 
-Require Import Psatz.
-Tactic Notation "math_nia" := math_setup; nia.
+Definition succ_using_incr :=
+  Fun 'n :=
+    Let 'p := 'ref 'n in
+    incr 'p ';
+    '! 'p.
 
-Lemma is_prime_spec : forall n,
-  n >= 2 ->
-  app is_prime [n]
+Lemma Triple_succ_using_incr : forall n,
+  TRIPLE (succ_using_incr ``n)
     PRE \[]
-    POST (fun (b:bool) => \[b = isTrue (prime n)]).
+    POST (fun r => \[r = n+1]).
 Proof using.
-  introv Hn. xcf. xapps. xapps.
-  xwhile_inv_basic (fun b k => Hexists vp,
-          \[b = isTrue (vp = true /\ k*k <= n)]
-       \* \[if vp then (forall d, 1 < d < k -> Z.rem n d <> 0) else (~ prime n)]
-       \* \[2 <= k]
-       \* i ~~> k
-       \* p ~~> vp)
-    (upto n).
-  { xsimpl. math. math. eauto. }
-  { => b k. xpull ;=> vp Hb Hp Hk. xapps. xand.
-    { xapps. xapps. xrets*. }
-    { xsimpl*. } }
-  { => k. xpull ;=> vp Hb Hp Hk.
-    xclean. (* cleans up results of boolean tests *)
-    destruct Hb as (Hvp&Hkk).
-    xapps. xapps. math.
-    xrets.
-    xseq. (* TODO: later try to change xif to remove xseq *)
-    xif (# Hexists (vp':bool), i ~~> k \* p ~~> vp' \*
-       \[if vp' then (forall d, 1 < d < (k+1) -> Z.rem n d <> 0) else (~ prime n)]).
-      { xapps. xsimpl. applys~ divide_not_prime. math_nia. }
-      { xrets. rewrite Hvp in *. =>> Hd. tests: (d = k). auto. applys~ Hp. }
-    xpull ;=> vp' Hvp'. xapps. xsimpl.
-    { math. }
-    { auto. }
-    { eauto. }
-    { math_nia. } }
-  => k vp Hb Hvp Hk. xclean. rew_logic in Hb.
-  xapps. xsimpl. subst. case_if; rew_bool_eq.
-  { destruct Hb; tryfalse. applys* not_divide_prime_sqrt. math. }
-  { auto. }
+  xwp. xapp ;=> p. (* xapp. intros p. *)
+  xapp. xapp. xsimpl*.
 Qed.
 
+(** Note: [decr] is similarly defined in the library. *)
 
-(***********************************************************************)
-(** Recursion *)
 
-(*---------------------------------------------------------------------*)
+
+(* ******************************************************* *)
+(** *** Increment with two references *)
 
 (**
 [[
-  let rec facto_rec n =
-    if n <= 1
-      then 1
-      else n * facto_rec(n-1)
+  let incr_one_of_two p q =
+    incr p
 ]]
 *)
 
-Lemma facto_rec_spec : forall n,
-  n >= 1 ->
-  app facto_rec [n]
-    PRE \[]
-    POST (fun (v:int) => \[v = facto n]).
+Definition incr_one_of_two : val :=
+  Fun 'p 'q :=
+    incr 'p.
+
+Lemma Triple_incr_one_of_two :
+  forall (p q:loc) (n m:int),
+  TRIPLE (incr_one_of_two p q)
+    PRE (p ~~> n \* q ~~> m)
+    POST (fun (r:unit) => p ~~> (n+1) \* q ~~> m).
 Proof using.
-  => n. induction_wf IH: (downto 0) n. unfolds downto. => Hn.
-  xcf. xif.
-  { xrets. math_rewrite (n=1). rewrite~ facto_one. }
-  { xapps. math. math. (* optimization: could be written [xapps~] *)
-    xrets. rewrite~ (@facto_succ n). }
+  xwp. xapp. xsimpl.
 Qed.
 
 
-(*---------------------------------------------------------------------*)
+(* ******************************************************* *)
+(** *** Increment and allocate a copy *)
 
 (**
 [[
-  let rec fib_rec n =
-    if n <= 1
-      then 1
-      else fib_rec(n-1) + fib_rec(n-2)
+  let incr_and_ref p =
+    incr p;
+    ref !p
 ]]
 *)
 
-Lemma fib_rec_spec : forall n,
+Definition incr_and_ref : val :=
+  Fun 'p :=
+    incr 'p ';
+    'ref ('! 'p).
+
+Lemma Triple_incr_and_ref : forall (p:loc) (n:int),
+  TRIPLE (incr_and_ref p)
+    PRE (p ~~> n)
+    POST (fun (q:loc) => q ~~> (n+1) \* p ~~> (n+1)).
+Proof using.
+  xwp. xapp. xapp. xapp. xsimpl.
+Qed.
+
+Hint Extern 1 (Register_Spec (incr_and_ref)) => Provide Triple_incr_and_ref.
+
+Lemma Triple_incr_and_ref' : forall (p:loc) (n:int),
+  TRIPLE (incr_and_ref p)
+    PRE (p ~~> n)
+    POST (fun (q:loc) =>
+        \exists m, \[m > n] \* q ~~> m \* p ~~> (n+1)).
+Proof using.
+  xtriple. xapp. intros q. xsimpl. math.
+Qed.
+
+
+(* ******************************************************* *)
+(** *** A simple recursion *)
+
+(**
+[[
+  let rec repeat_incr p m =
+    if m > 0 then (
+      incr p;
+      repeat_incr p (m-1)
+    )
+]]
+*)
+
+Definition repeat_incr :=
+  Fix 'f 'p 'm :=
+    If_ 'm '> 0 Then
+      incr 'p ';
+      'f 'p ('m '- 1)
+    (* Else '() *) End.
+
+(** Let's try to prove a false specification *)
+
+Lemma Triple_repeat_incr : forall p n m,
+  TRIPLE (repeat_incr p m)
+    PRE (p ~~> n)
+    POST (fun (_:unit) => p ~~> (n + m)).
+Proof using.
+  intros. gen n. induction_wf IH: (downto 0) m. intros.
+  xwp. xapp. xif ;=> C.
+  { (* then branch *)
+    xapp. xapp. xapp. { unfold downto. math. } xsimpl. math. }
+  { (* else branch *)
+    xval. xsimpl.
+Abort.
+
+(** Let's try again *)
+
+Lemma Triple_repeat_incr : forall p n m,
+  m >= 0 ->
+  TRIPLE (repeat_incr p m)
+    PRE (p ~~> n)
+    POST (fun (_:unit) => p ~~> (n + m)).
+Proof using.
+  introv Hm. gen n Hm. induction_wf IH: (downto 0) m. intros.
+  xwp. xapp. xif; intros C.
+  { xapp. xapp. xapp. { hnf. math. } { math. }
+    xsimpl. math. }
+  { xval. xsimpl. math. }
+Qed.
+
+(** Let's try yet another time *)
+
+Lemma Triple_repeat_incr' : forall p n m,
+  TRIPLE (repeat_incr p m)
+    PRE (p ~~> n)
+    POST (fun (_:unit) => p ~~> (n + max 0 m)).
+Proof using.
+  intros. gen n. induction_wf IH: (downto 0) m; intros.
+  xwp. xapp. xif; intros C.
+  { xapp. xapp. xapp. { hnf. math. }
+    xsimpl. repeat rewrite max_nonneg; math. }
+  { xval. xsimpl. rewrite max_nonpos; math. }
+Qed.
+
+(** Note: [xif] calls [xapp] if necessary. *)
+
+End Basics.
+
+
+(* ####################################################### *)
+(** * Entailment tactic *)
+
+Module XsimplDemo.
+
+(* ******************************************************* *)
+(** *** [xpull] to extract from LHS *)
+
+Lemma xpull_demo_hpure : forall H1 H2 n,
+  H1 \* \[n = 3] ==> H2.
+Proof using.
+  intros. xpull. intros Hn.
+Abort.
+
+Lemma xpull_demo_hexists : forall H1 H2 p,
+  H1 \* \exists (n:int), (p ~~> n) ==> H2.
+Proof using.
+  intros. xpull. intros n.
+Abort.
+
+Lemma xpull_demo_lhs_several : forall H1 H2 H3 H4 p q,
+  H1 \* \exists (n:int), (p ~~~> n \* \[n > 0] \* H2) \* \[p <> q] \* H3 ==> H4.
+Proof using.
+  intros. xpull. intros n Hn Hp. (* or [xpull ;=> n Hn Hp] *)
+Abort.
+
+
+(* ******************************************************* *)
+(** *** [xsimpl] to cancel out heap predicates from LHS and RHS *)
+
+(** For example, [H2] occurs on both sides, so it can be cancelled out. *)
+
+Lemma xsimpl_demo_cancel_one : forall H1 H2 H3 H4 H5 H6 H7,
+  H1 \* H2 \* H3 \* H4 ==> H5 \* H6 \* H2 \* H7.
+Proof using.
+  intros. xsimpl.
+Abort.
+
+(** [xsimpl] can cancel several predicates, here [H2], [H3], and [H4]. *)
+
+Lemma xsimpl_demo_cancel_many : forall H1 H2 H3 H4 H5,
+  H1 \* H2 \* H3 \* H4 ==> H4 \* H3 \* H5 \* H2.
+Proof using.
+  intros. xsimpl.
+Abort.
+
+(** If all the pieces get cancelled out, then the goal is discharged. *)
+
+Lemma xsimpl_demo_cancel_all : forall H1 H2 H3 H4,
+  H1 \* H2 \* H3 \* H4 ==> H4 \* H3 \* H1 \* H2.
+Proof using.
+  intros. xsimpl.
+Qed.
+
+(** [xsimpl] cancels what remains with the [\GC] from the RHS. *)
+
+Lemma xsimpl_demo_rhs_hgc : forall H1 H2 H3 H4,
+  H1 \* H2 \* H3 \* H4 ==> H3 \* H2 \* \GC.
+Proof using.
+  intros. xsimpl.
+Abort.
+
+
+(* ******************************************************* *)
+(** *** [xsimpl] to instantiate pure facts and quantifiers in RHS *)
+
+(** [xsimpl] instantiates existential quantifiers, pure facts,
+    and [\Top] in the RHS. *)
+
+Lemma xsimpl_demo_rhs_hpure : forall H1 H2 H3 (n:int),
+  H1 ==> H2 \* \[n > 0] \* H3.
+Proof using.
+  intros. xsimpl.
+Abort.
+
+(** For existentials, [xsimpl] introduces an evar. *)
+
+Lemma xsimpl_demo_rhs_hexists : forall H1 H2 H3 H4 (p:loc),
+  H1 ==> H2 \* \exists (n:int), (p ~~> n \* H3) \* H4.
+Proof using.
+  intros. xsimpl. (* here, [p ~~> n] becomes [p ~~> ?x] *)
+Abort.
+
+(** The evar often gets subsequently instantiated during cancellation. *)
+
+Lemma xsimpl_demo_rhs_hexists_unify : forall H1 H2 H3 H4 (p:loc),
+  H1 \* (p ~~> 3) ==>
+  H2 \* \exists (n:int), (p ~~> n \* H3) \* H4.
+Proof using.
+  intros. xsimpl. (* [p ~~~> n] becomes [p ~~~> ?x],
+                     which then cancels out with [p ~~~> 3] *)
+Abort.
+
+
+(* ******************************************************* *)
+(** ** The [xchange] tactic *)
+
+(** [xchange] is to entailment what [rewrite] is to equality. *)
+
+(** Assume an entailment goal of the form [H1 \* H2 \* H3 ==> H4].
+    Assume an entailment assumption [M], say [H2 ==> H2'].
+    Then [xchange M] turns the goal into [H1 \* H2' \* H3 ==> H4],
+    effectively replacing [H2] with [H2']. *)
+
+Lemma xchange_demo_base : forall H1 H2 H2' H3 H4,
+  H2 ==> H2' ->
+  H1 \* H2 \* H3 ==> H4.
+Proof using.
+  introv M. xchange M. (* Note that freshly produced items appear to the front *)
+Abort.
+
+(** The tactic [xchange] can also take as argument equalities.
+    Use [xchange M] to exploit the left-to-right direction
+    and [xchange <- M] to exploit the right-to-left direction . *)
+
+Lemma xchange_demo_eq : forall H1 H2 H3 H4 H5,
+  H1 \* H3 = H5 ->
+  H1 \* H2 \* H3 ==> H4.
+Proof using.
+  introv M. xchange M.
+  xchange <- M.
+Abort.
+
+(** The tactic [xchanges M] is a shorthand for [xchange M; xsimpl]. *)
+
+End XsimplDemo.
+
+
+
+(* ####################################################### *)
+(** * Hands-on: basic functions *)
+
+Module ExoBasic.
+
+(** Hints:
+    - [xwp] to begin the proof
+    - [xapp] for applications, or [xappn] to repeat
+    - [xif] for a case analysis
+    - [xval] for a value
+    - [xsimpl] to prove entailments
+    - [auto], [math], [rew_list] to prove pure facts
+      or just [*] after a tactic to invoke automation.
+*)
+
+
+(* ******************************************************* *)
+(** ** Basic pure function (warm up) *)
+
+(**
+[[
+  let double n =
+    n + n
+]]
+*)
+
+Definition double :=
+  Fun 'n :=
+    'n '+ 'n.
+
+Lemma Triple_double : forall n,
+  TRIPLE (double n)
+    PRE \[]
+    POST (fun m => (* SOLUTION *) \[m = 2 * n] (* /SOLUTION *)).
+Proof using.
+  (* SOLUTION *) xwp. xapp. xsimpl. math. (* /SOLUTION *)
+Qed.
+
+
+(* ******************************************************* *)
+(** ** Basic imperative function with one argument *)
+
+(**
+[[
+  let inplace_double p =
+    p := !p + !p
+]]
+*)
+
+Definition inplace_double :=
+  Fun 'p :=
+    'p ':= ('!'p '+ '!'p).
+
+Lemma Triple_inplace_double : forall p n,
+  TRIPLE (inplace_double p)
+    PRE ((* SOLUTION *) p ~~> n (* /SOLUTION *))
+    POST (fun (_:unit) => (* SOLUTION *) p ~~> (2 * n) (* /SOLUTION *)).
+Proof using.
+  (* SOLUTION *) xwp. xapp. xapp. xapp. xapp. xsimpl. math. (* /SOLUTION *)
+Qed.
+
+
+(* ******************************************************* *)
+(** ** Basic imperative function with two arguments (white belt) *)
+
+(**
+[[
+  let decr_and_incr p q =
+    decr p;
+    incr q
+]]
+*)
+
+Definition decr_and_incr :=
+  Fun 'p 'q :=
+    decr 'p ';
+    incr 'q.
+
+Lemma Triple_decr_and_incr : forall p q n m,
+  TRIPLE (decr_and_incr p q)
+    PRE ((* SOLUTION *) p ~~> n \* q ~~> m (* /SOLUTION *))
+    POST ((* SOLUTION *) fun (_:unit) => p ~~> (n-1) \* q ~~> (m+1) (* /SOLUTION *)).
+Proof using.
+  (* SOLUTION *) xwp. xapp. xapp. xsimpl. (* /SOLUTION *)
+Qed.
+
+
+(* ******************************************************* *)
+(** *** A recursive function (yellow belt) *)
+
+(** Here, we will assume [!p > 0].
+
+[[
+  let rec transfer p q =
+    if !p > 0 then (
+      decr p;
+      incr q;
+      transfer p q
+    )
+]]
+*)
+
+Definition transfer :=
+  Fix 'f 'p 'q :=
+    If_ '! 'p '> 0 Then
+      decr 'p ';
+      incr 'q ';
+      'f 'p 'q
+    End.
+
+Lemma Triple_transfer : forall p q n m,
   n >= 0 ->
-  app fib_rec [n]
-    PRE \[]
-    POST (fun (v:int) => \[v = fib n]).
+  TRIPLE (transfer p q)
+    PRE (p ~~> n \* q ~~> m)
+    POST (fun (_:unit) => (* SOLUTION *) p ~~> 0 \* q ~~> (n + m) (* /SOLUTION *)).
 Proof using.
-  (* Hint: follow the pattern for the previous example *)
-  (* <EXO> *)
-  => n. induction_wf IH: (downto 0) n. => Hn.
-  xcf. xif.
-  { xrets. rewrite~ fib_base. }
-  { xapps~. xapps~. xrets. rewrite~ (@fib_succ n). }
-  (* </EXO> *)
+  introv N. gen m N. induction_wf IH: (downto 0) n. intros.
+  (* SOLUTION *)
+  xwp. xapp. xapp. xif ;=> C.
+  { xapp. xapp. xapp. { hnf. math. } { math. }
+    xsimpl. math. }
+  { xval. xsimpl. math. math. }
+  (* /SOLUTION *)
 Qed.
 
-
-
-(***********************************************************************)
-(** Stack *)
-
-(*---------------------------------------------------------------------*)
-
-(*
-[[
-  module StackList = struct
-
-    type 'a t = {
-       mutable items : 'a list;
-       mutable size : int }
-
-    let create () =
-      { items = [];
-        size = 0 }
-
-    let size s =
-      s.size
-
-    let is_empty s =
-      s.size = 0
-
-    let push x s =
-      s.items <- x :: s.items;
-      s.size <- s.size + 1
-
-    let pop s =
-      match s.items with
-      | hd::tl ->
-          s.items <- tl;
-          s.size <- s.size - 1;
-          hd
-      | [] -> assert false
-
-  end
-]]
-*)
-
-Module StackListProof.
-
-Import StackList_ml.
-
-
-(** Definition of [r ~> Stack L], which is a notation for [Stack L r] of type [hprop] *)
-
-Definition Stack A (L:list A) r :=
-  Hexists n,
-      r ~> `{ items' := L; size' := n }
-   \* \[ n = length L ].
-
-(** Unfolding and folding lemmas paraphrasing the definition of [Stack] *)
-
-Lemma Stack_open : forall r A (L:list A),
-  r ~> Stack L ==>
-  Hexists n, r ~> `{ items' := L; size' := n } \* \[ n = length L ].
-Proof using. dup 2.
-  { intros. xunfold Stack. hpull. intros. hcancel. auto.
-    (* Try [hcancel 3] to see how it works *) }
-  { intros. xunfolds~ Stack. }
-Qed.
-
-
-Lemma Stack_close : forall r A (L:list A) (n:int),
-  n = length L ->
-  r ~> `{ items' := L; size' := n } ==>
-  r ~> Stack L.
-Proof using. intros. xunfolds~ Stack. Qed.
-
-Arguments Stack_close : clear implicits.
-
-
-(** Customization of [xopen] and [xclose] tactics for [Stack].
-    These tactics avoid the need to call [hchange] or [xchange]
-    by providing explicitly the lemmas [Stack_open] and [Stack_close].
-    Note that the number of underscores avec [Stack] after the [RegisterOpen]
-    needs to match the number of arguments of the representation predicate
-    [Stack], excluding the pointer. (Here, we have one underscore for [L].) *)
-
-Hint Extern 1 (RegisterOpen (Stack _)) =>
-  Provide Stack_open.
-Hint Extern 1 (RegisterClose (record_repr _)) =>
-  Provide Stack_close.
-
-
-(** Verification of the code *)
-
-Lemma create_spec : forall (A:Type),
-  app create [tt]
-    PRE \[]
-    POST (fun r => r ~> Stack (@nil A)).
-Proof using.
-  xcf. dup 2.
-  { xapp. intros r.  (* or just [xapp. => r] *)
-    xclose r. auto. xsimpl. }
-  { xapp ;=> r. xclose~ r. }
-Qed.
-
-Lemma size_spec : forall (A:Type) (L:list A) (s:loc),
-  app size [s]
-    INV (s ~> Stack L)
-    POST (fun n => \[n = length L]).
-(* Remark: the above is a notation for:
-  app size [s]
-    PRE (s ~> Stack L)
-    POST (fun n => \[n = length L] \* s ~> Stack L).
-*)
-Proof using.
-  xcf. (* TODO: add xopens to do xpull *)
-  xopen s. (* details: xchange (@Stack_open s). *)
-  xpull ;=> n Hn.
-  (* interesting: do [unfold tag] here, to unfold this identity
-     function used to decorate the file. *)
-  xapp. (* computes on-the-fly the record_get specification *)
-  intros m.
-  xpull ;=> ->. (* details: [xpull. intros E. subst E.] *)
-  xclose s. (* details: xchange (@Stack_close s). *)
-  auto. xsimpl. math.
-  (* Here we have an issue because Coq is a bit limited.
-     Workaround to discharge the remaining type: *)
-  Unshelve. solve_type. (* TODO: support [xcf A] in the beginning *)
-Qed.
-
-Lemma length_zero_iff_nil : forall A (L:list A),
-  length L = 0 <-> L = nil.
-Proof using.
-  intros. destruct L; rew_list. (* [rew_list] normalizes list expressions *)
-  { autos*. (* [intuition eauto] *) }
-  { iff M; false; math. (* [iff M] is [split; intros M] *) }
-Qed.
-
-Lemma is_empty_spec : forall (A:Type) (L:list A) (s:loc),
-  (* <EXO> *)
-  app is_empty [s]
-    INV (s ~> Stack L)
-    POST (fun b => \[b = isTrue (L = nil)]).
-  (* </EXO> *)
-Proof using.
-  (* Hint: use [xopen] then [xclose] like in [size_spec].
-     Also use [xcf], [xpull], [xapps], [xrets],
-     and lemma [length_zero_iff_nil] from above. *)
-  (* <EXO> *)
-  xcf.
-  (* Note that the boolean expression [n = 0] from Caml
-     was automatically translated into [isTrue (x0__ = 0)];
-     Indeed, [Ret_ P] is notation for [Ret (isTrue P)]. *)
-  xopen s. xpull ;=> n Hn. xapps. xclose~ s.
-  dup 2.
-  { xret_no_clean.
-    reflect_clean tt. (* automatically called by [hsimpl] *)
-    hsimpl.
-    subst. apply length_zero_iff_nil. }
-  { xrets. subst. apply length_zero_iff_nil. }
-  (* </EXO> *)
-  Unshelve. solve_type.
-Qed.
-
-Lemma push_spec : forall (A:Type) (L:list A) (s:loc) (x:A),
-  app push [x s]
-    PRE (s ~> Stack L)
-    POST (# s ~> Stack (x::L)).
-Proof using.
-  (* Hint: use [xcf], [xapp], [xapps], [xpull], [xsimpl],
-     [xopen], [xclose] and [rew_list] *)
-  (* <EXO> *)
-  xcf.
-  xopen s. (* details: xchange (@Stack_open s) *)
-  xpull ;=> n Hn.
-  xapps. xapp.
-  xapps. xapp.
-  xclose s. (* details: xchange (@Stack_close s) *)
-  rew_list. (* normalizes expression on lists *)
-  math.
-  xsimpl.
-  (* </EXO> *)
-Qed.
-
-Hint Extern 1 (RegisterSpec push) => Provide push_spec.
-
-(* [xapp] on a call to push.
-   Otherwise, need to do [xapp_spec push_spec]. *)
-
-Lemma pop_spec : forall (A:Type) (L:list A) (s:loc),
-  L <> nil ->
-  app pop [s]
-    PRE (s ~> Stack L)
-    POST (fun x => Hexists L', \[L = x::L'] \* s ~> Stack L').
-Proof using.
-  (* Hint: also use [rew_list in H] *)
-  (* <EXO> *)
-  =>> HL. xcf. xopen s. xpull ;=> n Hn. xapps. xmatch.
-  xapps. xapps. xapps. xret. xclose~ s. rew_list in Hn. math.
-  (* </EXO> *)
-Qed.
-
-
-
-(***********************************************************************)
-(** Array *)
-
-(*---------------------------------------------------------------------*)
-(*
-[[
-  let demo_array () =
-    let t = Array.make 3 true in
-    t.(0) <- false;
-    t.(1) <- false;
-    t
-]]
-*)
-
-Lemma demo_array_spec :
-  app demo_array [tt]
-    PRE \[]
-    POST (fun (t:loc) => Hexists M, (t ~> Array M)
-       \* \[forall k, 0 <= k < 3 -> M[k] = isTrue(k > 1)]).
-Proof using.
-  dup 2.
-  { (* Detailed proof: *)
-    xcf.
-    xapp. math. => M EM.
-    xapp. autos.
-    xapp. autos.
-    xret. xsimpl. =>> Hk. subst M. rew_array; autos.
-     case_ifs. math. math. math. }
-  { (* Shorter proof *)
-    xcf. xapp~. => M EM. xapp~. xapp~. xrets.
-    =>> Hk. subst M. rew_array~. case_ifs; math. }
-Qed.
-
-
-
-(*---------------------------------------------------------------------*)
-(*
-[[
-  let exercise_array () =
-    let t = Array.make 3 true in
-    t.(2) <- false;
-    t.(1) <- t.(2);
-    t
-]]
-*)
-
-Lemma exercise_array_spec :
-  App exercise_array tt;
-    \[]
-    (fun (t:loc) => Hexists M, (t ~> Array M) \*
-      \[length M = 3
-    /\ forall k, 0 <= k < 3 -> M[k] = isTrue(k<1)]).
-Proof using.
-  xcf.
-  xapp. autos. intros M EM. subst M.
-  xapp. autos.
-  xapp~ as v. intros Ev.
-  xapp~.
-  xret.
-  xsimpl. split.
-    rew_array~.
-    introv Hk. rew_array~. case_ifs.
-      subst v. rew_array~. case_if~. math.
-      math.
-      math.
-  (* Optional forward reasoning after [intros Ev]:
-    asserts Ev': (v = false).
-      subst. rew_array~. case_if~.
-      clear Ev. subst v. *)
-Qed.
-
-
-
-
-
-(***********************************************************************)
-(***********************************************************************)
-(***********************************************************************)
-
-End StackListProof.
-
-
-
-(* LATER
-  Hint Resolve length_nonneg : maths.
-  Hint Extern 1 (length (?l[?i:=?v]) = _) => rewrite length_update.
-  Hint Resolve length_make : maths.
-  Hint Extern 1 (length ?M = _) => subst M : maths.
-  Hint Constructors Forall.
-  Global Opaque Z.mul.
-*)
+End ExoBasic.
