examples/Stack/StackSized_proof.v
@@ -1,0 +1,189 @@
+(** See theories/ExampleStack.v for corresponding formalization in the deep embedding. *)
+
+Set Implicit Arguments.
+From CFML Require Import CFLib.
+Generalizable Variables A.
+
+Implicit Types n m : int.
+Implicit Types p q : loc.
+
+Import StackList_ml.
+
+
+(* ********************************************************************** *)
+(** ** Representation predicate *)
+
+(** Definition of [r ~> Stack L], which is a notation for [Stack L r], of type
+    [hprop] *)
+
+Definition Stack A (L:list A) r :=
+  \exists n,
+      r ~> `{ items' := L; size' := n }
+   \* \[ n = length L ].
+
+
+Lemma Stack_eq : forall r A (L:list A),
+  (r ~> Stack L) =
+  (\exists n, r ~> `{ items' := L; size' := n } \* \[ n = length L ]).
+Proof using. auto. Qed.
+
+Arguments Stack_eq : clear implicits.
+
+Tactic Notation "xopen" constr(r) :=
+  rewrite (Stack_eq r); xpull.
+
+Tactic Notation "xclose" constr(r) :=
+  rewrite <- (Stack_eq r).
+
+
+(* ********************************************************************** *)
+(** ** TEMPORARY *)
+
+(* TODO: generalize tactics using:
+
+  (** Unfolding and folding lemmas paraphrasing the definition of [Stack] *)
+
+  Lemma Stack_open : forall r A (L:list A),
+    r ~> Stack L ==>
+    \exists n, r ~> `{ items' := L; size' := n } \* \[ n = length L ].
+  Proof using. dup 2.
+    { intros. xunfold Stack. hpull. intros. hcancel. auto.
+      (* Try [hcancel 3] to see how it works *) }
+    { intros. xunfolds~ Stack. }
+  Qed.
+
+  Lemma Stack_close : forall r A (L:list A) (n:int),
+    n = length L ->
+    r ~> `{ items' := L; size' := n } ==>
+    r ~> Stack L.
+  Proof using. intros. xunfolds~ Stack. Qed.
+
+  Arguments Stack_close : clear implicits.
+
+  (** Customization of [xopen] and [xclose] tactics for [Stack].
+      These tactics avoid the need to call [hchange] or [xchange]
+      by providing explicitly the lemmas [Stack_open] and [Stack_close].
+      Note that the number of underscores avec [Stack] after the [RegisterOpen]
+      needs to match the number of arguments of the representation predicate
+      [Stack], excluding the pointer. (Here, we have one underscore for [L].) *)
+
+  Hint Extern 1 (RegisterOpen (Stack _)) =>
+    Provide Stack_open.
+  Hint Extern 1 (RegisterClose (record_repr _)) =>
+    Provide Stack_close.
+
+*)
+
+
+(* ********************************************************************** *)
+(** ** Verification *)
+
+(** Verification of the code *)
+
+Lemma create_spec : forall (A:Type),
+  TRIPLE (create tt)
+    PRE \[]
+    POST (fun r => r ~> Stack (@nil A)).
+Proof using.
+  xwp. dup 2.
+  { xapp. intros r.  (* or just [xapp. => r] *)
+    xclose r. auto. xsimpl. }
+  { xapp ;=> r. xclose~ r. }
+Qed.
+
+Lemma size_spec : forall (A:Type) (L:list A) (s:loc),
+  TRIPLE (size s)
+    INV (s ~> Stack L)
+    POST (fun n => \[n = length L]).
+(* Remark: the above is a notation for:
+  app size [s]
+    PRE (s ~> Stack L)
+    POST (fun n => \[n = length L] \* s ~> Stack L).
+*)
+Proof using.
+  xwp. (* TODO: add xopens to do xpull *)
+  xopen s. (* details: xchange (@Stack_open s). *)
+  xpull ;=> n Hn.
+  (* interesting: do [unfold tag] here, to unfold this identity
+     function used to decorate the file. *)
+  xapp. (* computes on-the-fly the record_get specification *)
+  intros m.
+  xpull ;=> ->. (* details: [xpull. intros E. subst E.] *)
+  xclose s. (* details: xchange (@Stack_close s). *)
+  auto. xsimpl. math.
+  (* Here we have an issue because Coq is a bit limited.
+     Workaround to discharge the remaining type: *)
+  Unshelve. solve_type. (* TODO: support [xwp A] in the beginning *)
+Qed.
+
+Lemma length_zero_iff_nil : forall A (L:list A),
+  length L = 0 <-> L = nil.
+Proof using.
+  intros. destruct L; rew_list. (* [rew_list] normalizes list expressions *)
+  { autos*. (* [intuition eauto] *) }
+  { iff M; false; math. (* [iff M] is [split; intros M] *) }
+Qed.
+
+Lemma is_empty_spec : forall (A:Type) (L:list A) (s:loc),
+  (* <EXO> *)
+  TRIPLE (is_empty s)
+    INV (s ~> Stack L)
+    POST (fun b => \[b = isTrue (L = nil)]).
+  (* </EXO> *)
+Proof using.
+  (* Hint: use [xopen] then [xclose] like in [size_spec].
+     Also use [xwp], [xpull], [xapps], [xrets],
+     and lemma [length_zero_iff_nil] from above. *)
+  (* <EXO> *)
+  xwp.
+  (* Note that the boolean expression [n = 0] from Caml
+     was automatically translated into [isTrue (x0__ = 0)];
+     Indeed, [Ret_ P] is notation for [Ret (isTrue P)]. *)
+  xopen s. xpull ;=> n Hn. xapps. xclose~ s.
+  dup 2.
+  { xret_no_clean.
+    reflect_clean tt. (* automatically called by [hsimpl] *)
+    hsimpl.
+    subst. apply length_zero_iff_nil. }
+  { xrets. subst. apply length_zero_iff_nil. }
+  (* </EXO> *)
+  Unshelve. solve_type.
+Qed.
+
+Lemma push_spec : forall (A:Type) (L:list A) (s:loc) (x:A),
+  TRIPLE (push x s)
+    PRE (s ~> Stack L)
+    POST (# s ~> Stack (x::L)).
+Proof using.
+  (* Hint: use [xwp], [xapp], [xapps], [xpull], [xsimpl],
+     [xopen], [xclose] and [rew_list] *)
+  (* <EXO> *)
+  xwp.
+  xopen s. (* details: xchange (@Stack_open s) *)
+  xpull ;=> n Hn.
+  xapps. xapp.
+  xapps. xapp.
+  xclose s. (* details: xchange (@Stack_close s) *)
+  rew_list. (* normalizes expression on lists *)
+  math.
+  xsimpl.
+  (* </EXO> *)
+Qed.
+
+Hint Extern 1 (RegisterSpec push) => Provide push_spec.
+
+(* [xapp] on a call to push.
+   Otherwise, need to do [xapp_spec push_spec]. *)
+
+Lemma pop_spec : forall (A:Type) (L:list A) (s:loc),
+  L <> nil ->
+  TRIPLE (pop s)
+    PRE (s ~> Stack L)
+    POST (fun x => \exists L', \[L = x::L'] \* s ~> Stack L').
+Proof using.
+  (* Hint: also use [rew_list in H] *)
+  (* <EXO> *)
+  introv HL. xwp. xopen s. xpull ;=> n Hn. xapps. xmatch.
+  xapps. xapps. xapps. xret. xclose~ s. rew_list in Hn. math.
+  (* </EXO> *)
+Qed.
