examples/Stack/Stack_proof.v
@@ -1,0 +1,107 @@
+(** See theories/ExampleStack.v for corresponding formalization in the deep embedding. *)
+
+Set Implicit Arguments.
+From CFML Require Import CFLib.
+Generalizable Variables A.
+
+Implicit Types n m : int.
+Implicit Types p q : loc.
+
+Import StackList_ml.
+
+
+(* ********************************************************************** *)
+(** ** Representation predicate *)
+
+(** [p ~> Stack L] relates a pointer [p] with the list [L] made of
+    the elements in the stack. *)
+
+Definition Stack A `{Enc A} (L:list A) (p:loc) : hprop :=
+  p ~~> L.
+
+
+(* ********************************************************************** *)
+(** ** Verification *)
+
+Lemma Triple_create : forall A `{Enc A},
+  TRIPLE (create '())
+    PRE \[]
+    POST (fun p => (p ~> Stack (@nil A))).
+Proof using.
+  xwp. xval. xapp. xsimpl.
+Qed.
+
+Hint Extern 1 (Register_Spec create) => Provide Triple_create.
+
+Lemma Triple_is_empty : forall A `{Enc A} (p:loc) (L:list A),
+  TRIPLE (is_empty p)
+    PRE (p ~> Stack L)
+    POST (fun (b:bool) => \[b = isTrue (L = nil)] \* p ~> Stack L).
+Proof using.
+  xwp. xunfold Stack. xapp. xval. xapp~. xsimpl*.
+Qed.
+
+Hint Extern 1 (Register_Spec is_empty) => Provide Triple_is_empty.
+
+Lemma Triple_push : forall A `{Enc A} (p:loc) (x:A) (L:list A),
+  TRIPLE (push p (``x))
+    PRE (p ~> Stack L)
+    POST (fun (u:unit) => (p ~> Stack (x::L))).
+Proof using.
+  xwp. xunfold Stack. xapp. xval. xapp. xsimpl.
+Qed.
+
+Hint Extern 1 (Register_Spec push) => Provide Triple_push.
+
+Lemma Triple_pop : forall A `{Enc A} (p:loc) (L:list A),
+  L <> nil ->
+  TRIPLE (pop p)
+    PRE (p ~> Stack L)
+    POST (fun (x:A) => \exists L', \[L = x::L'] \* (p ~> Stack L')).
+Proof using.
+  introv N. xwp. xunfold Stack. xapp.
+  applys xmatch_lemma_list.
+  { intros HL. xfail. }
+  { intros X L' HL. xapp. xval. xsimpl~. }
+Qed.
+
+Hint Extern 1 (Register_Spec pop) => Provide Triple_pop.
+
+Lemma Triple_clear : forall A `{Enc A} (p:loc) (L:list A),
+  TRIPLE (clear p)
+    PRE (p ~> Stack L)
+    POSTUNIT (p ~> Stack (@nil A)).
+Proof using.
+  xwp. xunfold Stack. xval. xapp. xapp. xsimpl.
+Qed.
+
+Hint Extern 1 (Register_Spec clear) => Provide Triple_clear.
+
+Lemma Triple_concat : forall A `{Enc A} (p1 p2:loc) (L1 L2:list A),
+  TRIPLE (concat p1 p2)
+    PRE (p1 ~> Stack L1 \* p2 ~> Stack L2)
+    POST (fun (u:unit) => p1 ~> Stack (L1 ++ L2) \* p2 ~> Stack (@nil A)).
+Proof using.
+  xwp. xunfold Stack. xapp. xapp. xapp. xapp. xapp. xapp. xapp.
+  xapp. { rew_listx. auto. } xapp. xsimpl.
+Qed.
+
+Hint Extern 1 (Register_Spec concat) => Provide @riple_concat.
+
+Opaque Stack.
+
+Lemma Triple_rev_append : forall A `{Enc A} (p1 p2:loc) (L1 L2:list A),
+  TRIPLE (rev_append p1 p2)
+    PRE (p1 ~> Stack L1 \* p2 ~> Stack L2)
+    POSTUNIT (p1 ~> Stack (@nil A) \* p2 ~> Stack (rev L1 ++ L2)).
+Proof using.
+  intros. gen p1 p2 L2. induction_wf IH: (@list_sub A) L1. intros.
+  xwp. xapp. xapp. xif ;=> C.
+  { (* case cons *)
+    xapp~ ;=> x L1' E. xapp. xapp. { subst*. } xsimpl. subst. rew_list~. }
+  { (* case nil *)
+    xval. xsimpl~. subst. rew_list~. }
+Qed.
+
+Hint Extern 1 (Register_Spec rev_append) => Provide Triple_rev_append.
+
