examples/Tutorial/OldTutorial_proof.v
@@ -1,0 +1,826 @@
+Set Implicit Arguments.
+Require Import CFML.CFLib.
+Require Import Stdlib.
+Require Import Array_proof.
+Require Import Tuto_ml.
+Require Import TLC.LibListZ.
+
+
+(***********************************************************************)
+(** Cheat list *)
+
+(**
+Specification syntax:
+   - [TRIPLE (f x y)
+        PRE H
+        POST (fun (r:T) => H']
+
+Heap syntax H :  heap -> Prop ::=
+   - \[]
+   - \[P]
+   - H \* H'
+   - r ~~> v        r ~> Ref v       Ref v r
+   - r ~~> (v+1)
+   - \exists x, H
+   - r ~> Stack L       Stack L r
+
+Coq tactics:
+   - [=> x], [=>> H], [exists v]
+   - [rew_maths] for normalizing math expressions
+   - [rew_list] for normalizing list operations
+   - [autos], [math], [ring], [math_nia]
+
+CFML tactics:
+   - [xwp]
+   - [xsimpl], or [xsimpl X1 .. X2] (to instantiate Hexists)
+   - [xpull]
+   - [xclean] sometimes needed to do simplifications (TODO:update)
+   - [xret], or [xrets] for substitution/simplification
+   - [xapp], or [xapps] for substitution
+   - [xfor_inv (fun i => H)]
+   - [xwhile_inv_basic (fun b k => [b = isTrue(..)] \* H) (downto n)]
+   - [xif Q]
+   - [xmatch]
+
+Shortcut:  (TODO: update)
+   - [xpulls] like [xpull; intros x; subst x]
+   - [xrets] like [xret; xsimpl]
+   - [xapps] like [xapp; xpulls]
+   - [tactic~] like [tactic; eauto with maths]
+*)
+
+
+(***********************************************************************)
+(** Mathematical definitions *)
+
+(** Factorial *)
+
+Parameter facto : int -> int.
+Parameter facto_zero : facto 0 = 1.
+Parameter facto_one : facto 1 = 1.
+Parameter facto_succ : forall n, n >= 1 -> facto n = n * facto(n-1).
+
+(** Fibonnaci *)
+
+Parameter fib : int -> int.
+Parameter fib_base : forall n, n <= 1 -> fib n = n.
+Parameter fib_succ : forall n, n > 1 -> fib n = fib(n-1) + fib(n-2).
+
+(** Primes *)
+
+Parameter prime : int -> Prop.
+Parameter divide_not_prime : forall n d,
+  1 < d < n ->
+  Z.rem n d = 0 ->
+  ~ (prime n).
+Parameter not_divide_prime : forall n,
+  (forall d, 1 < d < n -> Z.rem n d <> 0) ->
+  (prime n).
+Parameter not_divide_prime_sqrt : forall n r,
+  (forall d, 1 < d < r -> Z.rem n d <> 0) ->
+  (r * r > n) ->
+  (prime n).
+
+
+(***********************************************************************)
+(** Automation for mathematical subgoals *)
+
+Ltac auto_tilde ::= try solve [ intuition eauto with maths ].
+  (* TODO: try to use jauto *)
+
+Hint Extern 1 (index ?M _) => subst M : maths.
+Hint Resolve LibListZ.index_make : maths.
+Hint Resolve index_of_inbound : maths.
+Hint Resolve index_of_index_length int_index_prove : maths.
+Hint Resolve index_update : maths.
+
+(** Tactic [rew_maths] for simplifying math expressions *)
+
+Lemma math_plus_one_twice : forall n, ((n+1)+1) = n+2.
+Proof using. math. Qed.
+Lemma math_minus_same : forall n, n-n = 0.
+Proof using. math. Qed.
+Lemma math_two_minus_one : 2-1 = 1.
+Proof using. math. Qed.
+Lemma math_plus_minus_same : forall n m, (n+m)-m = n.
+Proof using. math. Qed.
+Hint Rewrite math_plus_one_twice math_minus_same
+  math_two_minus_one math_plus_minus_same : rew_maths.
+
+
+
+(***********************************************************************)
+(** Basic operations *)
+
+(*---------------------------------------------------------------------*)
+
+(**
+[[
+  let example_let n =
+    let a = n+1 in
+    let b = n-1 in
+    a + b
+]]
+*)
+
+Lemma example_let_spec : forall n,
+  TRIPLE (example_let n)
+    PRE \[]
+    POST (fun (v:int) => \[v = 2*n]).
+   (* post-condition also written: POST \[= (2 * n)]  *)
+Proof using.
+  (* Hint: the proof uses [xcf], [xret], [xsimpl], [math].
+     [xlet] is optional; if used then [xpull] is also needed. *)
+  dup 3.
+  { (* detailed proof *)
+    xcf.
+    xlet. xret. simpl. xpull. intros Ha.
+    xlet. xret. simpl. xpull. intros Hb.
+    xret. (*hnf.*) xsimpl. math. }
+  { (* shorter proof *)
+    xcf. xret ;=> Ha. xret ;=> Hb. xret. xsimpl. math. }
+  { (* real proof *)
+    xcf. xrets. xrets. xrets. math. }
+Qed.
+
+
+(*---------------------------------------------------------------------*)
+
+(**
+[[
+  let example_incr r =
+    r := !r + 1
+]]
+
+normalized to:
+
+[[
+  let example_incr r =
+    let x0__ := get r in
+    set r (x0__ + 1)
+]]
+*)
+
+Lemma example_incr_spec : forall r n,
+  TRIPLE (example_incr r)
+    PRE (r ~~> n)
+    POST (fun (_:unit) => (r ~~> (n+1))).
+    (* post-condition also written: POST (# r ~~> (n+1)). *)
+Proof using.
+  (* Hint: the proof uses [xcf], [xapp].
+     [xapps] is a shortand for [xapp] followed with [subst]. *)
+  dup 3.
+  { xcf. xlet. xapp. simpl. xpull. intros. subst. xapp. }
+  { xcf. xapp. intros. subst. xapp. }
+  { xcf. xapps. xapp. }
+Qed.
+
+(* Note: recall the specifications of get and set from Pervasives_proof:
+
+  Lemma get_spec : forall A (v:A) r,
+    app get [r]
+      PRE (r ~~> v)
+      POST (fun x => \[x = v] \* r ~~> v)
+
+  Lemma set_spec : forall A (v w:A) r,
+    app set [r w] (r ~~> v) (# r ~~> w).
+
+*)
+
+(*---------------------------------------------------------------------*)
+
+(**
+[[
+let example_two_ref n =
+  let i = ref 0 in
+  let r = ref n in
+  decr r;
+  incr i;
+  r := !i + !r;
+  !i + !r
+]]
+*)
+
+Lemma example_two_ref_spec : forall n: int,
+  (* <EXO> *)
+  TRIPLE (example_two_ref n)
+     PRE \[]
+     POST (fun x: int => \[ x = n+1 ]).
+  (* </EXO *)
+Proof using.
+  (* Hint: the proof uses [xcf], [xapp], [xapps], and [xret] or [xrets]. *)
+  dup 3.
+  { (* detailed proof *)
+    xcf.
+    xapp. (* details: xlet. xapp. simpl. *)
+    xapp. xapp. xapp.
+    xapps. (* details: xapp. intro. subst. *)
+    xapps. xapps. xapps. xapps.
+    xrets. (* details: xret. xsimpl. *)
+    math. }
+  { (* shorter proof, not recommended for nontrivial code *)
+    xcf. xgo. subst. math. }
+  { (* real proof *)
+    xcf. xgo~. }
+Qed.
+
+
+
+(***********************************************************************)
+(** For loops *)
+
+(*---------------------------------------------------------------------*)
+
+(**
+[[
+  let facto_for n =
+    let r = ref 1 in
+    for i = 1 to n do
+      r := !r * i;
+    done;
+    !r
+]]
+*)
+
+(* Reasoning principle for the loop [for i = a to b to t done] when [b+1>=a]
+   implemented by tactic [xfor_inv I].
+
+  I a               initial invariant
+
+  I i -> I (i+1)    when executing [t] on some [i] in the range from [a] to [b]
+
+  I (b+1)           final invariant
+
+*)
+
+Lemma facto_for_spec : forall n,
+  n >= 1 ->
+  TRIPLE (facto_for n)
+    PRE \[]
+    POST (fun (v:int) => \[v = facto n]).
+Proof using.
+  =>> Hn. xcf. xapps.
+  xfor_inv (fun i => r ~~> (facto (i-1))).
+  { math. }
+  { xsimpl. forwards: facto_zero. easy. }
+  { =>> Hi. xapps. xapps. xsimpl.
+    rew_maths. rewrite (@facto_succ i). ring. math. }
+  xapps. xsimpl. rew_maths. auto.
+Qed.
+
+
+
+(*---------------------------------------------------------------------*)
+
+(**
+[[
+  let fib_for n =
+    let a = ref 0 in
+    let b = ref 1 in
+    for i = 0 to n-1 do
+      let c = !a + !b in
+      a := !b;
+      b := c;
+    done;
+    !a
+]]
+*)
+
+Lemma fib_for_spec : forall n,
+  n >= 1 ->
+  TRIPLE (fib_for n)
+    PRE \[]
+    POST (fun (v:int) => \[v = fib n]).
+Proof using.
+  (* Hint: follow the pattern from the previous example *)
+  (* <EXO> *)
+  =>> Hn. xcf. xapps. xapps.
+  xfor_inv (fun i => a ~~> (fib i) \* b ~~> (fib (i+1)) ).
+  { math. }
+  { xsimpl.
+    rewrite~ fib_base. (* details: math. math. rewrite fib_base. *)
+    rewrite~ fib_base. }
+  { =>> Hi. xapps. xapps. xrets. xapps. xapps. xapps. xsimpl.
+    rew_maths. rewrite~ (@fib_succ (i+2)). rew_maths.
+    math_rewrite ((i + 2)-1 = i+1). math. }
+  xapps. xsimpl~.
+  (* </EXO> *)
+Qed.
+
+
+(*----Alternative script:
+
+  =>> Hn. xcf. xapps. xapps.
+  xfor_inv (fun i => a ~~> (fib i) \* b ~~> (fib (i+1))).
+  { math. }
+  { xsimpl.
+    { forwards~: fib_base. math. }
+    { forwards~: fib_base. math. } }
+  { introv Hi. xapps. xapps. xret. intros. xapps. xapps. xapps. xsimpl.
+    rewrite fib_succ. rew_maths. math. math. }
+  xapps. xsimpl. auto.
+*)
+
+
+
+(***********************************************************************)
+(** While loops *)
+
+(*---------------------------------------------------------------------*)
+
+(**
+[[
+  let example_while n =
+    let i = ref 0 in
+    let r = ref 0 in
+    while !i < n do
+      incr i;
+      incr r;
+    done;
+    !r
+]]
+*)
+
+(* Reasoning principle for the loop [while t1 do t2] using an invariant
+   implemented by tactic [xwhile_inv_basic J W].
+
+  J b i             true for some boolean [b] and some initial index [k]
+
+  J b i             when executing [t1] on some [i]
+   ->
+  J b' i
+
+  J true i          when executing [t2] on some [i], should restablish the
+   ->               invariant for some [b'] and some [i'] smaller than [i]
+  J b' i'           w.r.t. [W], that is [W i' i].
+
+  J false i         for some [i] describes the final state
+
+*)
+
+
+Lemma example_while_spec : forall n,
+  n >= 0 ->
+  TRIPLE (example_while n)
+    PRE \[]
+    POST (fun (v:int) => \[v = n]).
+Proof using.
+  introv Hn. xcf. xapps. xapps.
+  xwhile_inv_basic (fun b k => \[b = isTrue (k < n)] \* \[k <= n] \* i ~~> k \* r ~~> k)
+    (upto n).
+  { xsimpl. eauto. eauto. }
+  { => b k. xpull. => Hb Hk. xapps. xrets. auto. autos*. } (* short for: xret; xsimpl. *)
+  { => k. xpull. => Hb Hk. xapps. xapps. xsimpl.
+    { math. }
+    { eauto. }
+    { hnf. math. } }
+  =>> Hb Hk. xclean. xapps. xsimpl. subst. math.
+Qed.
+
+
+(*---------------------------------------------------------------------*)
+
+(**
+[[
+  let facto_while n =
+    let r = ref 1 in
+    let i = ref 1 in
+    while !i <= n do
+      r := !i * !r;
+      incr i;
+    done;
+    !r
+]]
+*)
+
+Lemma facto_while_spec : forall n,
+  n >= 2 ->
+  TRIPLE (facto_while n)
+    PRE \[]
+    POST (fun (v:int) => \[v = facto n]).
+Proof using.
+  (* Hint: follow the pattern from previous example *)
+  (* <EXO> *)
+  introv Hn. xcf. xapps. xapps.
+  xwhile_inv_basic (fun b k => \[b = isTrue (k <= n)] \* \[2 <= k <= n+1]
+                               \* i ~~> k \* r ~~> (facto (k-1)))
+    (upto (n+1)).
+  { xsimpl. rew_maths. rewrite~ facto_one. math. eauto. }
+  { => b k. xpull. => Hb Hk. xapps. xrets. auto. autos*. } (* short for: xret; xsimpl. *)
+  { => k. xpull. => Hb Hk. xapps. xapps. xapps. xapps. xsimpl.
+    { rew_maths. rewrite (@facto_succ k). ring. math. }
+    { math. }
+    { eauto. }
+    { math. } }
+  =>> Hb Hk. xclean. xapps. xsimpl. subst. fequal. math.
+  (* </EXO> *)
+Qed.
+
+
+(*---------------------------------------------------------------------*)
+
+(* TODO: add demos using the other xfor and xwhile approach *)
+
+(*---------------------------------------------------------------------*)
+
+(**
+[[
+  let is_prime n =
+    let i = ref 2 in
+    let p = ref true in
+    while !p && (!i * !i <= n) do
+      if (n mod !i) = 0
+        then p := false;
+      incr i;
+    done;
+    !p
+]]
+*)
+
+Require Import Psatz.
+Tactic Notation "math_nia" := math_setup; nia.
+
+Lemma is_prime_spec : forall n,
+  n >= 2 ->
+  TRIPLE (is_prime n)
+    PRE \[]
+    POST (fun (b:bool) => \[b = isTrue (prime n)]).
+Proof using.
+  introv Hn. xcf. xapps. xapps.
+  xwhile_inv_basic (fun b k => Hexists vp,
+          \[b = isTrue (vp = true /\ k*k <= n)]
+       \* \[if vp then (forall d, 1 < d < k -> Z.rem n d <> 0) else (~ prime n)]
+       \* \[2 <= k]
+       \* i ~~> k
+       \* p ~~> vp)
+    (upto n).
+  { xsimpl. math. math. eauto. }
+  { => b k. xpull ;=> vp Hb Hp Hk. xapps. xand.
+    { xapps. xapps. xrets*. }
+    { xsimpl*. } }
+  { => k. xpull ;=> vp Hb Hp Hk.
+    xclean. (* cleans up results of boolean tests *)
+    destruct Hb as (Hvp&Hkk).
+    xapps. xapps. math.
+    xrets.
+    xseq. (* TODO: later try to change xif to remove xseq *)
+    xif (# Hexists (vp':bool), i ~~> k \* p ~~> vp' \*
+       \[if vp' then (forall d, 1 < d < (k+1) -> Z.rem n d <> 0) else (~ prime n)]).
+      { xapps. xsimpl. applys~ divide_not_prime. math_nia. }
+      { xrets. rewrite Hvp in *. =>> Hd. tests: (d = k). auto. applys~ Hp. }
+    xpull ;=> vp' Hvp'. xapps. xsimpl.
+    { math. }
+    { auto. }
+    { eauto. }
+    { math_nia. } }
+  => k vp Hb Hvp Hk. xclean. rew_logic in Hb.
+  xapps. xsimpl. subst. case_if; rew_bool_eq.
+  { destruct Hb; tryfalse. applys* not_divide_prime_sqrt. math. }
+  { auto. }
+Qed.
+
+
+(***********************************************************************)
+(** Recursion *)
+
+(*---------------------------------------------------------------------*)
+
+(**
+[[
+  let rec facto_rec n =
+    if n <= 1
+      then 1
+      else n * facto_rec(n-1)
+]]
+*)
+
+Lemma facto_rec_spec : forall n,
+  n >= 1 ->
+  TRIPLE (facto_rec n)
+    PRE \[]
+    POST (fun (v:int) => \[v = facto n]).
+Proof using.
+  => n. induction_wf IH: (downto 0) n. unfolds downto. => Hn.
+  xcf. xif.
+  { xrets. math_rewrite (n=1). rewrite~ facto_one. }
+  { xapps. math. math. (* optimization: could be written [xapps~] *)
+    xrets. rewrite~ (@facto_succ n). }
+Qed.
+
+
+(*---------------------------------------------------------------------*)
+
+(**
+[[
+  let rec fib_rec n =
+    if n <= 1
+      then 1
+      else fib_rec(n-1) + fib_rec(n-2)
+]]
+*)
+
+Lemma fib_rec_spec : forall n,
+  n >= 0 ->
+  TRIPLE (fib_rec n)
+    PRE \[]
+    POST (fun (v:int) => \[v = fib n]).
+Proof using.
+  (* Hint: follow the pattern for the previous example *)
+  (* <EXO> *)
+  => n. induction_wf IH: (downto 0) n. => Hn.
+  xcf. xif.
+  { xrets. rewrite~ fib_base. }
+  { xapps~. xapps~. xrets. rewrite~ (@fib_succ n). }
+  (* </EXO> *)
+Qed.
+
+
+
+(***********************************************************************)
+(** Stack *)
+
+(*---------------------------------------------------------------------*)
+
+(*
+[[
+  module StackList = struct
+
+    type 'a t = {
+       mutable items : 'a list;
+       mutable size : int }
+
+    let create () =
+      { items = [];
+        size = 0 }
+
+    let size s =
+      s.size
+
+    let is_empty s =
+      s.size = 0
+
+    let push x s =
+      s.items <- x :: s.items;
+      s.size <- s.size + 1
+
+    let pop s =
+      match s.items with
+      | hd::tl ->
+          s.items <- tl;
+          s.size <- s.size - 1;
+          hd
+      | [] -> assert false
+
+  end
+]]
+*)
+
+Module StackListProof.
+
+Import StackList_ml.
+
+
+(** Definition of [r ~> Stack L], which is a notation for [Stack L r] of type [hprop] *)
+
+Definition Stack A (L:list A) r :=
+  Hexists n,
+      r ~> `{ items' := L; size' := n }
+   \* \[ n = length L ].
+
+(** Unfolding and folding lemmas paraphrasing the definition of [Stack] *)
+
+Lemma Stack_open : forall r A (L:list A),
+  r ~> Stack L ==>
+  Hexists n, r ~> `{ items' := L; size' := n } \* \[ n = length L ].
+Proof using. dup 2.
+  { intros. xunfold Stack. hpull. intros. hcancel. auto.
+    (* Try [hcancel 3] to see how it works *) }
+  { intros. xunfolds~ Stack. }
+Qed.
+
+
+Lemma Stack_close : forall r A (L:list A) (n:int),
+  n = length L ->
+  r ~> `{ items' := L; size' := n } ==>
+  r ~> Stack L.
+Proof using. intros. xunfolds~ Stack. Qed.
+
+Arguments Stack_close : clear implicits.
+
+
+(** Customization of [xopen] and [xclose] tactics for [Stack].
+    These tactics avoid the need to call [hchange] or [xchange]
+    by providing explicitly the lemmas [Stack_open] and [Stack_close].
+    Note that the number of underscores avec [Stack] after the [RegisterOpen]
+    needs to match the number of arguments of the representation predicate
+    [Stack], excluding the pointer. (Here, we have one underscore for [L].) *)
+
+Hint Extern 1 (RegisterOpen (Stack _)) =>
+  Provide Stack_open.
+Hint Extern 1 (RegisterClose (record_repr _)) =>
+  Provide Stack_close.
+
+
+(** Verification of the code *)
+
+Lemma create_spec : forall (A:Type),
+  app create [tt]
+    PRE \[]
+    POST (fun r => r ~> Stack (@nil A)).
+Proof using.
+  xcf. dup 2.
+  { xapp. intros r.  (* or just [xapp. => r] *)
+    xclose r. auto. xsimpl. }
+  { xapp ;=> r. xclose~ r. }
+Qed.
+
+Lemma size_spec : forall (A:Type) (L:list A) (s:loc),
+  app size [s]
+    INV (s ~> Stack L)
+    POST (fun n => \[n = length L]).
+(* Remark: the above is a notation for:
+  app size [s]
+    PRE (s ~> Stack L)
+    POST (fun n => \[n = length L] \* s ~> Stack L).
+*)
+Proof using.
+  xcf. (* TODO: add xopens to do xpull *)
+  xopen s. (* details: xchange (@Stack_open s). *)
+  xpull ;=> n Hn.
+  (* interesting: do [unfold tag] here, to unfold this identity
+     function used to decorate the file. *)
+  xapp. (* computes on-the-fly the record_get specification *)
+  intros m.
+  xpull ;=> ->. (* details: [xpull. intros E. subst E.] *)
+  xclose s. (* details: xchange (@Stack_close s). *)
+  auto. xsimpl. math.
+  (* Here we have an issue because Coq is a bit limited.
+     Workaround to discharge the remaining type: *)
+  Unshelve. solve_type. (* TODO: support [xcf A] in the beginning *)
+Qed.
+
+Lemma length_zero_iff_nil : forall A (L:list A),
+  length L = 0 <-> L = nil.
+Proof using.
+  intros. destruct L; rew_list. (* [rew_list] normalizes list expressions *)
+  { autos*. (* [intuition eauto] *) }
+  { iff M; false; math. (* [iff M] is [split; intros M] *) }
+Qed.
+
+Lemma is_empty_spec : forall (A:Type) (L:list A) (s:loc),
+  (* <EXO> *)
+  app is_empty [s]
+    INV (s ~> Stack L)
+    POST (fun b => \[b = isTrue (L = nil)]).
+  (* </EXO> *)
+Proof using.
+  (* Hint: use [xopen] then [xclose] like in [size_spec].
+     Also use [xcf], [xpull], [xapps], [xrets],
+     and lemma [length_zero_iff_nil] from above. *)
+  (* <EXO> *)
+  xcf.
+  (* Note that the boolean expression [n = 0] from Caml
+     was automatically translated into [isTrue (x0__ = 0)];
+     Indeed, [Ret_ P] is notation for [Ret (isTrue P)]. *)
+  xopen s. xpull ;=> n Hn. xapps. xclose~ s.
+  dup 2.
+  { xret_no_clean.
+    reflect_clean tt. (* automatically called by [hsimpl] *)
+    hsimpl.
+    subst. apply length_zero_iff_nil. }
+  { xrets. subst. apply length_zero_iff_nil. }
+  (* </EXO> *)
+  Unshelve. solve_type.
+Qed.
+
+Lemma push_spec : forall (A:Type) (L:list A) (s:loc) (x:A),
+  app push [x s]
+    PRE (s ~> Stack L)
+    POST (# s ~> Stack (x::L)).
+Proof using.
+  (* Hint: use [xcf], [xapp], [xapps], [xpull], [xsimpl],
+     [xopen], [xclose] and [rew_list] *)
+  (* <EXO> *)
+  xcf.
+  xopen s. (* details: xchange (@Stack_open s) *)
+  xpull ;=> n Hn.
+  xapps. xapp.
+  xapps. xapp.
+  xclose s. (* details: xchange (@Stack_close s) *)
+  rew_list. (* normalizes expression on lists *)
+  math.
+  xsimpl.
+  (* </EXO> *)
+Qed.
+
+Hint Extern 1 (RegisterSpec push) => Provide push_spec.
+
+(* [xapp] on a call to push.
+   Otherwise, need to do [xapp_spec push_spec]. *)
+
+Lemma pop_spec : forall (A:Type) (L:list A) (s:loc),
+  L <> nil ->
+  app pop [s]
+    PRE (s ~> Stack L)
+    POST (fun x => Hexists L', \[L = x::L'] \* s ~> Stack L').
+Proof using.
+  (* Hint: also use [rew_list in H] *)
+  (* <EXO> *)
+  =>> HL. xcf. xopen s. xpull ;=> n Hn. xapps. xmatch.
+  xapps. xapps. xapps. xret. xclose~ s. rew_list in Hn. math.
+  (* </EXO> *)
+Qed.
+
+
+
+(***********************************************************************)
+(** Array *)
+
+(*---------------------------------------------------------------------*)
+(*
+[[
+  let demo_array () =
+    let t = Array.make 3 true in
+    t.(0) <- false;
+    t.(1) <- false;
+    t
+]]
+*)
+
+Lemma demo_array_spec :
+  app demo_array [tt]
+    PRE \[]
+    POST (fun (t:loc) => Hexists M, (t ~> Array M)
+       \* \[forall k, 0 <= k < 3 -> M[k] = isTrue(k > 1)]).
+Proof using.
+  dup 2.
+  { (* Detailed proof: *)
+    xcf.
+    xapp. math. => M EM.
+    xapp. autos.
+    xapp. autos.
+    xret. xsimpl. =>> Hk. subst M. rew_array; autos.
+     case_ifs. math. math. math. }
+  { (* Shorter proof *)
+    xcf. xapp~. => M EM. xapp~. xapp~. xrets.
+    =>> Hk. subst M. rew_array~. case_ifs; math. }
+Qed.
+
+
+
+(*---------------------------------------------------------------------*)
+(*
+[[
+  let exercise_array () =
+    let t = Array.make 3 true in
+    t.(2) <- false;
+    t.(1) <- t.(2);
+    t
+]]
+*)
+
+Lemma exercise_array_spec :
+  App exercise_array tt;
+    \[]
+    (fun (t:loc) => Hexists M, (t ~> Array M) \*
+      \[length M = 3
+    /\ forall k, 0 <= k < 3 -> M[k] = isTrue(k<1)]).
+Proof using.
+  xcf.
+  xapp. autos. intros M EM. subst M.
+  xapp. autos.
+  xapp~ as v. intros Ev.
+  xapp~.
+  xret.
+  xsimpl. split.
+    rew_array~.
+    introv Hk. rew_array~. case_ifs.
+      subst v. rew_array~. case_if~. math.
+      math.
+      math.
+  (* Optional forward reasoning after [intros Ev]:
+    asserts Ev': (v = false).
+      subst. rew_array~. case_if~.
+      clear Ev. subst v. *)
+Qed.
+
+
+
+
+
+(***********************************************************************)
+(***********************************************************************)
+(***********************************************************************)
+
+End StackListProof.
+
+
+
+(* LATER
+  Hint Resolve length_nonneg : maths.
+  Hint Extern 1 (length (?l[?i:=?v]) = _) => rewrite length_update.
+  Hint Resolve length_make : maths.
+  Hint Extern 1 (length ?M = _) => subst M : maths.
+  Hint Constructors Forall.
+  Global Opaque Z.mul.
+*)
