lib/coq/CFLib.v
@@ -8,9 +8,10 @@ Require Export CFHeader (* CFBuiltin TODO? *) CFTactics.
 
 
 
-
-(* ---------------------------------------------------------------------- *)
-(** Additional notation for more concise specifications at scale. *)
+(* ********************************************************************** *)
+(* ********************************************************************** *)
+(* ********************************************************************** *)
+(** * Additional notation for more concise specifications at scale. *)
 
 (** The following notation is only used for parsing. *)
 
@@ -82,3 +83,190 @@ Notation "'TRIPLE' T 'PRE' H1 'INV'' H2 'RET' v 'POST' H3" :=
    format "'[v' 'TRIPLE'  t '/' '[' 'PRE''  H1  ']'  '/' '[' 'INV''  H2  ']'  '/' '[' 'RET'  v  'POST'  H3  ']'  ']'")
    : triple_scope.
 
+
+(* ********************************************************************** *)
+(* ********************************************************************** *)
+(* ********************************************************************** *)
+(** * Tactics for unfolding and folding representation predicates *)
+
+(* TODO *)
+
+(* ********************************************************************** *)
+(** ** Database *)
+
+(** The focus and unfocus databases are used to register specifications
+    for accessors to record fields, combined with focus/unfocus operations.
+    See example/Stack/StackSized_proof.v for a demo of this feature. *)
+
+Definition database_xopen := True.
+Definition database_xclose := True.
+
+Notation "'RegisterOpen' T" := (Register database_xopen T)
+  (at level 69) : charac.
+
+Notation "'RegisterClose' T" := (Register database_xclose T)
+  (at level 69) : charac.
+
+
+(* ********************************************************************** *)
+(** ** [xopen] *)
+
+(** [xopen] is a tactic for applying [xchange] without having
+    to explicitly specify the name of a focusing lemma.
+
+    [xopen p] applies to a goal of the form
+    [F H Q] or [H ==> H'] or [Q ===> Q'].
+    It first searches for the pattern [p ~> T] in the pre-condition,
+    then looks up in a database for the focus lemma [E] associated with
+    the form [T], and then calls [xchange E].
+
+    [xopen_show p] shows the lemma found, it is useful for debugging.
+
+    Example for registering a focusing lemma:
+      Hint Extern 1 (RegisterOpen (Tree _)) => Provide tree_open.
+    See [Demo_proof.v] for examples.
+
+    Then, use: [xopen p].
+
+    Variants:
+    - [xopenx t]  is short for [xopen t; xpull]
+
+    - [xopenxs t]  is short for [xopen t; xpulls]  // EXPERIMENTAL
+
+    - [xopen2 p] to perform [xopen p] twice. Only applies when there
+      is no existentials to be extracted after the first [xopen].
+
+*)
+
+Ltac get_refocus_args tt :=
+  match goal with
+  | |- ?Q1 ===> ?Q2 => constr:((Q1,Q2))
+  | |- ?H1 ==> ?H2 => constr:((H1,H2))
+  | |- ?R ?H1 ?Q2 => constr:((H1,Q2))
+  (* TODO: gérer le cas de fonctions appliquées à R *)
+  end.
+
+Ltac get_refocus_constr_in H t :=
+  match H with context [ t ~> ?T ] => constr:(T) end.
+
+Ltac xopen_constr t :=
+  match get_refocus_args tt with (?H1,?H2) =>
+  get_refocus_constr_in H1 t end.
+
+Ltac xopen_core t :=
+  let C1 := xopen_constr t in
+  ltac_database_get database_xopen C1;
+  let K := fresh "TEMP" in
+  intros K; xchange (K t); clear K.
+
+Ltac xopen_show_core t :=
+  let C1 := xopen_constr t in
+  pose C1;
+  try ltac_database_get database_xopen C1;
+  intros.
+
+Tactic Notation "xopen_show" constr(t) :=
+  xopen_show_core t.
+
+Tactic Notation "xopen" constr(t) :=
+  xopen_core t.
+Tactic Notation "xopen" "~" constr(t) :=
+  xopen t; xauto~.
+Tactic Notation "xopen" "*" constr(t) :=
+  xopen t; xauto*.
+
+Tactic Notation "xopen2" constr(x) :=
+  xopen x; xopen x.
+Tactic Notation "xopen2" "~" constr(x) :=
+  xopen2 x; xauto_tilde.
+Tactic Notation "xopen2" "*" constr(x) :=
+  xopen2 x; xauto_star.
+
+Tactic Notation "xopenx" constr(t) :=
+  xopen t; xpull.
+
+Tactic Notation "xopenxs" constr(t) :=
+  xopen t; xpulls.
+
+
+(* ********************************************************************** *)
+(** ** [xclose] *)
+
+(** [xclose] is the symmetrical of [xopen]. It works in the
+    same way, except that it looks for an unfocusing lemma.
+
+    [xclose p] applies to a goal of the form
+    [F H Q] or [H ==> H'] or [Q ===> Q'].
+    It first searches for the pattern [p ~> T] in the pre-condition,
+    then looks up in a database for the unfocus lemma [E] associated with
+    the form [T], and then calls [xchange E].
+
+    [xclose_show p] shows the lemma found, it is useful for debugging.
+
+    Example for registering a focusing lemma:
+
+     Hint Extern 1 (RegisterClose (Ref Id (MNode _ _ _))) =>
+        Provide tree_node_close.
+
+    Then, use: [xclose p].
+
+    Variants:
+
+    - [xclose p1 .. pn] is short for [xclose p1; ..; xclose pn]
+
+    - [xclose2 p] to perform [xclose p] twice.
+
+    - [xclose (>> p X Y)] where the extra arguments are used to
+      provide explicit arguments to instantiate the "closing" lemma.
+
+*)
+
+
+Ltac xclose_get_ptr args :=
+  match args with (boxer ?t)::_ => t end.
+
+Ltac xclose_constr args :=
+  let t := xclose_get_ptr args in
+  match get_refocus_args tt with (?H1,?H2) =>
+  get_refocus_constr_in H1 t end.
+
+Ltac xclose_core args :=
+  let args := list_boxer_of args in
+  let C1 := xclose_constr args in
+  ltac_database_get database_xclose C1;
+  let K := fresh "TEMP" in
+  intros K;
+  let E := constr:((boxer K)::args) in
+  xchange E;
+  clear K.
+
+Ltac xclose_show_core args :=
+  let args := list_boxer_of args in
+  let C1 := xclose_constr args in
+  pose C1;
+  try ltac_database_get database_xclose C1;
+  intros.
+
+Tactic Notation "xclose_show" constr(t) :=
+  xclose_show_core t.
+
+Tactic Notation "xclose" constr(t) :=
+  xclose_core t.
+Tactic Notation "xclose" "~" constr(t) :=
+  xclose t; xauto~.
+Tactic Notation "xclose" "*" constr(t) :=
+  xclose t; xauto*.
+
+Tactic Notation "xclose" constr(t1) constr(t2) :=
+  xclose t1; xclose t2.
+Tactic Notation "xclose" constr(t1) constr(t2) constr(t3) :=
+  xclose t1; xclose t2 t3.
+Tactic Notation "xclose" constr(t1) constr(t2) constr(t3) constr(t4) :=
+  xclose t1; xclose t2 t3 t4.
+
+Tactic Notation "xclose2" constr(x) :=
+  xclose x; xclose x.
+Tactic Notation "xclose2" "~" constr(x) :=
+  xclose2 x; xauto_tilde.
+Tactic Notation "xclose2" "*" constr(x) :=
+  xclose2 x; xauto_star.
